Progressing on insensitivity proof

cfrontend/SemanticsProofs.v
@@ -7,6 +7,7 @@ Require Import List. Import ListNotations.
 Require Import String.
 Require Import Coq.Logic.Eqdep_dec.
 Require Import NullPolicy.
+Require Import FunctionalExtensionality.
 
 Module PolicyInsensitivity (Ptr: Pointer) (Pol: Policy)
        (M: Memory Ptr) (A: Allocator Ptr).
@@ -39,30 +40,663 @@ Module PolicyInsensitivity (Ptr: Pointer) (Pol: Policy)
 
   Hypothesis globalenv1 :
     Csem1.globalenv prog1 = MemorySuccess (ge1,ce,m1).
+  Hypothesis globalenv2 :
+    Csem2.globalenv prog2 = MemorySuccess (ge2,ce,m2).
   
   Hypothesis sem1_src : Csem1.semantics prog1 ge1 ce = sem1.
   Hypothesis sem2_src : Csem2.semantics prog2 ge2 ce = sem2.
+
+  Module V1 := M1.MD.TLib.Switch.BI.BI1.BI0.Values.
+  Module V2 := M2.MD.TLib.Switch.BI.BI1.BI0.Values. 
+  
+  Definition vcoerce1 (v:V1.val) : V2.val :=
+    match v with
+    | V1.Vundef => V2.Vundef
+    | V1.Vint i => V2.Vint i
+    | V1.Vlong i => V2.Vlong i
+    | V1.Vfloat f => V2.Vfloat f
+    | V1.Vsingle f => V2.Vsingle f
+    | V1.Vptr p => V2.Vptr p
+    | V1.Vfptr b => V2.Vfptr b
+    | V1.Vefptr ef tyl rt cc => V2.Vefptr ef tyl rt cc
+    end.
+
+  Coercion vcoerce1 : V1.val >-> V2.val.
+
+  Definition match_val (v1: V1.val) (v2: V2.val) : Prop :=
+    v2 = v1.
+
+  Definition match_atom (v1: M1.MD.TLib.atom) (v2: M2.MD.TLib.atom) : Prop :=
+    match_val (fst v1) (fst v2).
+
+  Definition match_option_map {A1 A2:Type}
+             (m: A1 -> A2 -> Prop)
+             (a1: option A1) (a2: option A2) : Prop :=
+    match a1, a2 with
+    | Some a1', Some a2' => m a1' a2'
+    | None, None => True
+    | _, _ => False
+  end.
+
+  Fixpoint match_list_map {A1 A2:Type}
+             (m: A1 -> A2 -> Prop)
+             (al1: list A1) (al2: list A2) : Prop :=
+    match al1, al2 with
+    | a1::al1', a2::al2' =>
+        m a1 a2 /\ match_list_map m al1' al2'
+    | [], [] => True
+    | _, _ => False
+  end.
+
+  Inductive match_expr : CS1.expr -> CS2.expr -> Prop :=
+  | MEval : forall v1 v2 vt1 vt2 ty,
+      match_val v1 v2 ->
+      match_expr (CS1.Eval (v1,vt1) ty) (CS2.Eval (v2,vt2) ty)
+  | MEmloc : forall p bf pt1 pt2 ty,
+      match_expr (CS1.Eloc (CS1.Lmem p pt1 bf) ty)
+                 (CS2.Eloc (CS2.Lmem p pt2 bf) ty)      
+  | MEtloc : forall b ty,
+      match_expr (CS1.Eloc (CS1.Ltmp b) ty)
+                 (CS2.Eloc (CS2.Ltmp b) ty)      
+  | MEifloc : forall b pt1 pt2 ty,
+      match_expr (CS1.Eloc (CS1.Lifun b pt1) ty)
+                 (CS2.Eloc (CS2.Lifun b pt2) ty)      
+  | MEefloc : forall ef tyl rt cc pt1 pt2 ty,
+      match_expr (CS1.Eloc (CS1.Lefun ef tyl rt cc pt1) ty)
+                 (CS2.Eloc (CS2.Lefun ef tyl rt cc pt2) ty)
+  | MEparen : forall r1 r2 ty1 ty,
+      match_expr r1 r2 ->
+      match_expr (CS1.Eparen r1 ty1 ty) (CS2.Eparen r2 ty1 ty)
+  | MEvar : forall x ty,
+      match_expr (CS1.Evar x ty) (CS2.Evar x ty)
+  | MEconst : forall v1 v2 ty,
+      match_val v1 v2 ->
+      match_expr (CS1.Econst v1 ty) (CS2.Econst v2 ty)
+  | MEfield : forall l1 l2 f ty,
+      match_expr l1 l2 ->
+      match_expr (CS1.Efield l1 f ty) (CS2.Efield l2 f ty)
+  | MEvalof : forall l1 l2 ty,
+      match_expr l1 l2 ->
+      match_expr (CS1.Evalof l1 ty) (CS2.Evalof l2 ty)
+  | MEderef : forall r1 r2 ty,
+      match_expr r1 r2 ->
+      match_expr (CS1.Ederef r1 ty) (CS2.Ederef r2 ty)
+  | MEaddrof : forall l1 l2 ty,
+      match_expr l1 l2 ->
+      match_expr (CS1.Eaddrof l1 ty) (CS2.Eaddrof l2 ty)
+  | MEunop : forall op r1 r2 ty,
+      match_expr r1 r2 ->
+      match_expr (CS1.Eunop op r1 ty) (CS2.Eunop op r2 ty)
+  | MEbinop : forall op r1_1 r2_1 r1_2 r2_2 ty,
+      match_expr r1_1 r1_2 ->
+      match_expr r2_1 r2_2 ->
+      match_expr (CS1.Ebinop op r1_1 r2_1 ty) (CS2.Ebinop op r1_2 r2_2 ty)
+  | MEcast : forall r1 r2 ty,
+      match_expr r1 r2 ->
+      match_expr (CS1.Ecast r1 ty) (CS2.Ecast r2 ty)
+  | MEseqand : forall r1_1 r2_1 r1_2 r2_2 ty,
+      match_expr r1_1 r1_2 ->
+      match_expr r2_1 r2_2 ->
+      match_expr (CS1.Eseqand r1_1 r2_1 ty) (CS2.Eseqand r1_2 r2_2 ty)
+  | MEseqor : forall r1_1 r2_1 r1_2 r2_2 ty, 
+      match_expr r1_1 r1_2 ->
+      match_expr r2_1 r2_2 ->
+      match_expr (CS1.Eseqor r1_1 r2_1 ty) (CS2.Eseqor r1_2 r2_2 ty)
+  | MEcondition : forall r1_1 r2_1 r3_1 r1_2 r2_2 r3_2 ty,
+      match_expr r1_1 r1_2 ->
+      match_expr r2_1 r2_2 ->
+      match_expr r3_1 r3_2 ->
+      match_expr (CS1.Econdition r1_1 r2_1 r3_1 ty) (CS2.Econdition r1_2 r2_2 r3_2 ty)
+  | MEsizeof : forall ty' ty,  
+      match_expr (CS1.Esizeof ty' ty) (CS2.Esizeof ty' ty)
+  | MEalignof : forall ty' ty,       
+      match_expr (CS1.Ealignof ty' ty) (CS2.Ealignof ty' ty)
+  | MEassign : forall l1 l2 r1 r2 ty,
+      match_expr l1 l2 ->
+      match_expr r1 r2 ->
+      match_expr (CS1.Eassign l1 r1 ty) (CS2.Eassign l2 r2 ty)
+  | MEassignop : forall op l1 l2 r1 r2 tyres ty,
+      match_expr l1 l2 ->
+      match_expr r1 r2 ->
+      match_expr (CS1.Eassignop op l1 r1 tyres ty) (CS2.Eassignop op l2 r2 tyres ty)
+  | MEpostincr : forall l1 l2 ty,
+      match_expr l1 l2 ->
+      match_expr (CS1.Epostincr CS1.Cop.Incr l1 ty) (CS2.Epostincr CS2.Cop.Incr l2 ty)  | MEpostdecr : forall l1 l2 ty,
+      match_expr l1 l2 ->
+      match_expr (CS1.Epostincr CS1.Cop.Decr l1 ty) (CS2.Epostincr CS2.Cop.Decr l2 ty)
+  | MEcomma : forall r1_1 r2_1 r1_2 r2_2 ty,                  
+      match_expr r1_1 r1_2 ->
+      match_expr r2_1 r2_2 ->
+      match_expr (CS1.Ecomma r1_1 r2_1 ty) (CS2.Ecomma r1_2 r2_2 ty)
+  | MEcall : forall r1_1 r1_2 rargs1 rargs2 ty,
+      match_expr r1_1 r1_2 ->
+      match_exprlist rargs1 rargs2 ->
+      match_expr (CS1.Ecall r1_1 rargs1 ty) (CS2.Ecall r1_2 rargs2 ty)
+  | MEbuiltin : forall ef tyargs cc ty,
+      match_expr (CS1.Ebuiltin ef tyargs cc ty) (CS2.Ebuiltin ef tyargs cc ty)
+  with match_exprlist : CS1.exprlist -> CS2.exprlist -> Prop :=
+  | MEnil : match_exprlist CS1.Enil CS2.Enil
+  | MEcons : forall e1 e2 el1 el2,
+      match_expr e1 e2 ->
+      match_exprlist el1 el2 ->
+      match_exprlist (CS1.Econs e1 el1) (CS2.Econs e2 el2) 
+  .
+  
+  Inductive match_statement : CS1.statement -> CS2.statement -> Prop :=
+  | MSskip : match_statement CS1.Sskip CS2.Sskip
+  | MSSdo : forall e1 e2 l,
+      match_expr e1 e2 ->
+      match_statement (CS1.Sdo e1 l) (CS2.Sdo e2 l)
+  | MSsequence : forall s1_1 s2_1 s1_2 s2_2,
+        match_statement s1_1 s1_2 ->
+        match_statement s2_1 s2_2 ->
+        match_statement (CS1.Ssequence s1_1 s2_1) (CS2.Ssequence s1_2 s2_2)
+  | MSifthenelse : forall e1 e2 s1_1 s1_2 s2_1 s2_2 lb lc,
+      match_expr e1 e2 ->
+      match_statement s1_1 s1_2 ->
+      match_statement s2_1 s2_2 ->
+      match_statement (CS1.Sifthenelse e1 s1_1 s2_1 lb lc)
+                      (CS2.Sifthenelse e2 s1_2 s2_2 lb lc)
+  | MSwhile : forall e1 e2 s1 s2 lb lc,
+      match_expr e1 e2 ->
+      match_statement s1 s2 ->
+      match_statement (CS1.Swhile e1 s1 lb lc) (CS2.Swhile e2 s2 lb lc)
+  | MSdowhile : forall e1 e2 s1 s2 lb lc,
+      match_expr e1 e2 ->
+      match_statement s1 s2 ->
+      match_statement (CS1.Sdowhile e1 s1 lb lc) (CS2.Sdowhile e2 s2 lb lc)
+  | MSfor: forall s1_1 s1_2 e1 e2 s2_1 s2_2 s3_1 s3_2 lb lc,
+      match_statement s1_1 s1_2 ->
+      match_expr e1 e2 ->
+      match_statement s2_1 s2_2 ->
+      match_statement s3_1 s3_2 ->
+      match_statement (CS1.Sfor s1_1 e1 s2_1 s3_1 lb lc)
+                      (CS2.Sfor s1_2 e2 s2_2 s3_2 lb lc)                      
+  | MSbreak : forall l,
+      match_statement (CS1.Sbreak l) (CS2.Sbreak l)
+  | MScontinue : forall l,
+      match_statement (CS1.Scontinue l) (CS2.Scontinue l)
+  | MSreturn_Some : forall e1 e2 l,
+      match_expr e1 e2 ->
+      match_statement (CS1.Sreturn (Some e1) l) (CS2.Sreturn (Some e2) l)
+  | MSreturn_None : forall l,
+      match_statement (CS1.Sreturn None l) (CS2.Sreturn None l)     
+  | MSswitch : forall e1 e2 ls1 ls2 l,
+      match_expr e1 e2 ->
+      match_ls ls1 ls2 ->
+      match_statement (CS1.Sswitch e1 ls1 l) (CS2.Sswitch e2 ls2 l)
+  | MSlabel : forall l s1 s2,
+      match_statement s1 s2 ->
+      match_statement (CS1.Slabel l s1) (CS2.Slabel l s2)
+  | MSgoto : forall lb lc,
+      match_statement (CS1.Sgoto lb lc) (CS2.Sgoto lb lc)
+
+  with match_ls : CS1.labeled_statements -> CS2.labeled_statements -> Prop :=
+  | MLSnil: match_ls CS1.LSnil CS2.LSnil
+  | MLScons: forall z s1 s2 ls1 ls2,
+      match_statement s1 s2 ->
+      match_ls ls1 ls2 ->
+      match_ls (CS1.LScons z s1 ls1) (CS2.LScons z s2 ls2)
+  .
+
+  Inductive match_function : CS1.function ->
+                             CS2.function -> Prop :=
+    MFunc: forall fn_return fn_callconv fn_params fn_vars fn_body1 fn_body2,
+        match_statement fn_body1 fn_body2 ->
+        match_function (CS1.mkfunction fn_return fn_callconv fn_params fn_vars fn_body1)
+                       (CS2.mkfunction fn_return fn_callconv fn_params fn_vars fn_body2)
+  .
+  
+  Inductive match_var_entry : Csem1.var_entry -> Csem2.var_entry -> Prop :=
+  | MPRIV : forall ty,
+      match_var_entry (Csem1.PRIV ty) (Csem2.PRIV ty) 
+  | MPUB : forall p1 p2 pt1 pt2 ty,
+      match_var_entry (Csem1.PUB p1 p2 pt1 ty)
+                      (Csem2.PUB p1 p2 pt2 ty) 
+  .
+  
+  Definition match_env (e1: Csem1.env) (e2: Csem2.env) : Prop :=
+    forall p, match_option_map match_var_entry (e1!p) (e2!p).
+
+  Definition match_tenv (te1: Csem1.tenv) (te2: Csem2.tenv) : Prop :=
+    forall p, match_option_map match_atom (te1!p) (te2!p).
+
+  Definition coerce_kind1 (k: Csem1.kind) : Csem2.kind :=
+    match k with
+    | Csem1.LV => Csem2.LV
+    | Csem1.RV => Csem2.RV
+    end.
+
+  Definition coerce_kind2 (k: Csem2.kind) : Csem1.kind :=
+    match k with
+    | Csem2.LV => Csem1.LV
+    | Csem2.RV => Csem1.RV
+    end.
+
+  Coercion coerce_kind1 : Csem1.kind >-> Csem2.kind.
+  Coercion coerce_kind2 : Csem2.kind >-> Csem1.kind.
+  
+  Record match_ctx
+         (ctx1: CS1.expr -> CS1.expr)
+         (ctx2: CS2.expr -> CS2.expr) :=
+    ctxaxioms {
+        closed_expr : forall e1 e2,
+          match_expr e1 e2 ->
+          match_expr (ctx1 e1) (ctx2 e2);
+
+        r : forall e1 e2,
+          match_expr (ctx1 e1) e2 ->
+          exists e2',
+            e2 = ctx2 e2' /\ match_expr e1 e2';
+
+        l : forall e1 e2,
+          match_expr e1 (ctx2 e2) ->
+          exists e1',
+            e1 = ctx1 e1' /\ match_expr e1' e2;
+
+        closed_context : forall (k1_1 k2_1:Csem1.kind) (k1_2 k2_2:Csem2.kind),
+          k1_1 = k1_2 ->
+          k2_1 = k2_2 ->
+          (Csem1.context k1_1 k2_1 ctx1 <-> Csem2.context k1_2 k2_2 ctx2)
+      }.
+
+  Variable expr1_to_expr2 : CS1.expr -> CS2.expr.
+  Variable expr2_to_expr1 : CS2.expr -> CS1.expr.
+  
+  Definition matching_ctx (ctx1: CS1.expr -> CS1.expr) : CS2.expr -> CS2.expr :=
+    fun e2 =>
+      let e1 := expr2_to_expr1 e2 in
+      let e1' := ctx1 e1 in
+      expr1_to_expr2 e1'.
+
+  Axiom matching_ctx_matches : forall ctx1,
+      match_ctx ctx1 (matching_ctx ctx1). 
+  
+  Inductive match_cont : Csem1.cont -> Csem2.cont -> Prop :=
+  | MKstop: match_cont Csem1.Kstop Csem2.Kstop
+  | MKdo: forall k1 k2,
+      match_cont k1 k2 ->
+      match_cont (Csem1.Kdo k1) (Csem2.Kdo k2)
+  | MKseq: forall s1 s2 k1 k2,
+      match_statement s1 s2 ->
+      match_cont k1 k2 ->
+      match_cont (Csem1.Kseq s1 k1) (Csem2.Kseq s2 k2)
+  | MKifthenelse: forall s1_1 s1_2 s2_1 s2_2 l k1 k2,
+      match_statement s1_1 s1_2 ->
+      match_statement s2_1 s2_2 ->
+      match_cont k1 k2 ->
+      match_cont (Csem1.Kifthenelse s1_1 s2_1 l k1)
+                 (Csem2.Kifthenelse s1_2 s2_2 l k2)
+  | MKwhile1: forall e1 e2 s1 s2 lb lc k1 k2,
+      match_expr e1 e2 ->
+      match_statement s1 s2 ->
+      match_cont k1 k2 ->
+      match_cont (Csem1.Kwhile1 e1 s1 lb lc k1)
+                 (Csem2.Kwhile1 e2 s2 lb lc k2)
+  | MKwhile2: forall e1 e2 s1 s2 lb lc k1 k2,
+      match_expr e1 e2 ->
+      match_statement s1 s2 ->
+      match_cont k1 k2 ->
+      match_cont (Csem1.Kwhile2 e1 s1 lb lc k1)
+                 (Csem2.Kwhile2 e2 s2 lb lc k2)
+  | MKdowhile1: forall e1 e2 s1 s2 lb lc k1 k2,
+      match_expr e1 e2 ->
+      match_statement s1 s2 ->
+      match_cont k1 k2 ->
+      match_cont (Csem1.Kdowhile1 e1 s1 lb lc k1)
+                 (Csem2.Kdowhile1 e2 s2 lb lc k2)
+  | MKdowhile2: forall e1 e2 s1 s2 lb lc k1 k2,
+      match_expr e1 e2 ->
+      match_statement s1 s2 ->
+      match_cont k1 k2 ->
+      match_cont (Csem1.Kdowhile2 e1 s1 lb lc k1)
+                 (Csem2.Kdowhile2 e2 s2 lb lc k2)
+  | MKfor2: forall e1 e2 s1_1 s1_2 s2_1 s2_2 lb lc k1 k2,
+      match_expr e1 e2 ->
+      match_statement s1_1 s1_2 ->
+      match_statement s2_1 s2_2 ->
+      match_cont k1 k2 ->
+      match_cont (Csem1.Kfor2 e1 s1_1 s2_1 lb lc k1)
+                 (Csem2.Kfor2 e2 s1_2 s2_2 lb lc k2)
+  | MKfor3: forall e1 e2 s1_1 s1_2 s2_1 s2_2 lb lc k1 k2,
+      match_expr e1 e2 ->
+      match_statement s1_1 s1_2 ->
+      match_statement s2_1 s2_2 ->
+      match_cont k1 k2 ->
+      match_cont (Csem1.Kfor3 e1 s1_1 s2_1 lb lc k1)
+                 (Csem2.Kfor3 e2 s1_2 s2_2 lb lc k2)
+  | MKfor4: forall e1 e2 s1_1 s1_2 s2_1 s2_2 lb lc k1 k2,
+      match_expr e1 e2 ->
+      match_statement s1_1 s1_2 ->
+      match_statement s2_1 s2_2 ->
+      match_cont k1 k2 ->
+      match_cont (Csem1.Kfor4 e1 s1_1 s2_1 lb lc k1)
+                 (Csem2.Kfor4 e2 s1_2 s2_2 lb lc k2)
+  | MKswitch1: forall ls1 ls2 k1 k2,
+      match_ls ls1 ls2 ->
+      match_cont k1 k2 ->
+      match_cont (Csem1.Kswitch1 ls1 k1) (Csem2.Kswitch1 ls2 k2)
+  | MKswitch2: forall k1 k2,
+      match_cont k1 k2 ->
+      match_cont (Csem1.Kswitch2 k1) (Csem2.Kswitch2 k2)
+  | MKreturn: forall k1 k2,
+      match_cont k1 k2 ->
+      match_cont (Csem1.Kreturn k1) (Csem2.Kreturn k2)
+  | MKcall: forall f1 f2 e1 e2 te1 te2 l pct1 pct2 ctx1 ctx2 ty k1 k2,
+      match_function f1 f2 ->
+      match_env e1 e2 ->
+      match_tenv te1 te2 ->
+      match_ctx ctx1 ctx2 ->
+      match_cont k1 k2 ->
+      match_cont (Csem1.Kcall f1 e1 te1 l pct1 ctx1 ty k1)
+                 (Csem2.Kcall f2 e2 te2 l pct2 ctx2 ty k2)
+  .
+
+  Record match_mem (m1:GV1.mem) (m2:GV2.mem) :=
+    mkmatchm
+      {
+        load_all_agree : forall chunk p v1 vt1 lts1,
+          GV1.load_all chunk m1 p = MemorySuccess (v1,vt1,lts1) ->
+          exists v2 vt2 lts2, GV2.load_all chunk m2 p = MemorySuccess (v2,vt2,lts2)
+                              /\ match_val v1 v2
+      ;
+        load_agree : forall chunk p v1 vt1,
+          GV1.load chunk m1 p = MemorySuccess (v1,vt1) ->
+          exists v2 vt2, GV2.load chunk m2 p = MemorySuccess (v2,vt2)
+                         /\ match_val v1 v2
+      ;
+        load_ltags_agree : forall chunk p lts1,
+          GV1.load_ltags chunk m1 p = MemorySuccess lts1 ->
+          exists lts2, GV2.load_all chunk m2 p = MemorySuccess lts2;
+      }.
   
   (* Define matching relation on states that holds if they match except for tags.*)
-  Print Csem1.state.
   Inductive match_states : Csem1.state -> Csem2.state -> Prop :=
   | MState : forall f1 f2 pct1 pct2 stmt1 stmt2 k1 k2 e1 e2 te1 te2 m1 m2,
+      match_function f1 f2 ->
+      (* Ignore PCT *)
+      match_statement stmt1 stmt2 ->
+      match_cont k1 k2 ->
+      match_env e1 e2 ->
+      match_tenv te1 te2 ->
+      (* Memories match *)
       match_states (Csem1.State f1 pct1 stmt1 k1 e1 te1 m1)
                    (Csem2.State f2 pct2 stmt2 k2 e2 te2 m2)
   | MExprState : forall f1 f2 l pct1 pct2 expr1 expr2 k1 k2 e1 e2 te1 te2 m1 m2,
+      match_function f1 f2 ->
+      (* Ignore PCT *)
+      match_expr expr1 expr2 ->
+      match_cont k1 k2 ->
+      match_env e1 e2 ->
+      match_tenv te1 te2 ->
       match_states (Csem1.ExprState f1 l pct1 expr1 k1 e1 te1 m1)
                    (Csem2.ExprState f2 l pct2 expr2 k2 e2 te2 m2)      
   | MCallstate : forall fd1 fd2 l pct1 pct2 fpt1 fpt2 args1 args2 k1 k2 m1 m2,
+      fundef_match fd1 fd2 ->
+      (* Ignore tags *)
+      match_list_map match_atom args1 args2 ->
+      match_cont k1 k2 ->
       match_states (Csem1.Callstate fd1 l pct1 fpt1 args1 k1 m1)
                    (Csem2.Callstate fd2 l pct2 fpt2 args2 k2 m2)
   | MReturnState : forall fd1 fd2 l pct1 pct2 retv1 retv2 k1 k2 m1 m2,
+      fundef_match fd1 fd2 ->
+      (* Ignore tags *)
+      match_atom retv1 retv2 ->
+      match_cont k1 k2 ->
       match_states (Csem1.Returnstate fd1 l pct1 retv1 k1 m1)
                    (Csem2.Returnstate fd2 l pct2 retv2 k2 m2)  
   | MStuckstate : match_states Csem1.Stuckstate Csem2.Stuckstate
-  | Failstop : forall s2 msg failure,
-      match_states (Csem1.Failstop msg failure [])
+  | Failstop : forall s2 msg failure params,
+      match_states (Csem1.Failstop msg failure params)
                    s2
   .
+
+  Lemma bool_val_eq :
+    forall v1 v2 ty m1 m2,
+      match_val v1 v2 ->
+      Csem1.Csyntax.Cop.bool_val v1 ty m1 =
+        Csem2.Csyntax.Cop.bool_val v2 ty m2.
+  Proof.
+    intros. inv H.
+    unfold CS1.Cop.bool_val.
+    unfold CS2.Cop.bool_val.
+    unfold CS1.Cop.classify_bool.
+    unfold CS2.Cop.classify_bool.
+    unfold typeconv.
+    destruct ty; auto.
+    - destruct i; destruct v1; auto.
+    - destruct (remove_attributes (Tlong s a)); auto.
+      + destruct v1; auto.
+      + destruct v1; auto.
+      + destruct f; destruct v1; auto.
+      + destruct v1; auto.
+    - destruct (remove_attributes (Tfloat f a)); auto.
+      + destruct v1; auto.
+      + destruct v1; auto.
+      + destruct f0; destruct v1; auto.
+      + destruct v1; auto.
+    - destruct (remove_attributes (Tpointer ty a)); auto.
+      + destruct v1; auto.
+      + destruct v1; auto.
+      + destruct f; destruct v1; auto.
+      + destruct v1; auto.
+    - destruct v1; auto.
+    - destruct v1; auto.
+  Qed.
+
+  Lemma sem_cast_match :
+    forall v1 v2 ty ty' m1 m2,
+      match_val v1 v2 ->
+      match_option_map match_val
+                       (CS1.Cop.sem_cast v1 ty ty' m1)
+                       (CS2.Cop.sem_cast v2 ty ty' m2).
+  Proof.
+    intros. inv H.
+    unfold CS1.Cop.sem_cast.
+    unfold CS2.Cop.sem_cast.
+    destruct ty; destruct ty'; simpl; try constructor.
+    all: try (destruct i; constructor).
+    all: try (destruct f; constructor).
+    all: try (destruct i0; destruct v1; constructor).
+    all: try (destruct v1; constructor).
+    all: try (destruct f; destruct v1; constructor).
+    all: try (destruct v1; constructor).
+    all: try (destruct i; destruct v1; constructor).
+  Admitted.
+
+  Lemma deref_loc_match :
+    forall ty m1 m2 ofs pt1 pt2 bf tr1 v1 vt1 lts1,
+      match_mem m1 m2 ->
+      Csem1.deref_loc ge1 ty m1 ofs pt1 bf tr1 (MemorySuccess ((v1,vt1),lts1)) ->
+      exists tr2 v2 vt2 lts2,
+        Csem2.deref_loc ge2 ty m2 ofs pt2 bf tr2 (MemorySuccess ((v2,vt2),lts2)).
+  Proof.
+    intros. inv H0.
+    - assert (exists v2 vt2 lts2,
+                 CS2.Cop.Events.Genv.load_all chunk m4 ofs =
+                   MemorySuccess (v2, vt2, lts2)). { admit. }
+      destruct H0 as [v2 [vt2 [lts2 H0]]]. eexists. exists v2, vt2, lts2.
+      rewrite <- H0.
+      eapply Csem2.deref_loc_value; eauto.
+    - assert (exists tr2 v2 vt2,
+                 Csem2.Smallstep.Events.volatile_load ge2 chunk m4 ofs tr2
+                   (MemorySuccess (v2, vt2))). { admit. }
+      assert (exists lts2,
+                 CS2.Cop.Events.Genv.load_ltags chunk m4 ofs =
+                   MemorySuccess lts2). { admit. }
+      destruct H0 as [tr2 [v2 [vt2 H0]]].
+      destruct H1 as [lts H1].
+      exists tr2, v2, vt2, lts.
+      eapply Csem2.deref_loc_volatile; eauto.
+    - exists E2.E0, (V2.Vptr ofs), pt2, [].
+      eapply Csem2.deref_loc_reference; eauto.
+    - exists E2.E0, (V2.Vptr ofs), pt2, [].
+      eapply Csem2.deref_loc_copy; eauto.
+    - assert (exists v2 vt2 lts,
+                 CS2.Cop.load_bitfield ty sz sg pos width m4 ofs
+                                       (MemorySuccess (v2,vt2,lts))).
+      { admit. }
+      destruct H0 as [v2 [vt2 [lts2 H0]]].
+      exists E2.E0, v2, vt2, lts2.
+      eapply Csem2.deref_loc_bitfield; eauto.
+  Admitted.
+      
+  Ltac eexist' :=
+    match goal with
+    | [ |- exists _, _ ] => eexists
+    end.
+  
+  Ltac deduce_match :=
+    match goal with
+    | [ |- _ /\ _ /\ _ ] =>
+        intuition; [| econstructor; eauto | econstructor]
+    | [ |- _ /\ _ ] =>
+        intuition; [| econstructor; eauto ]
+    end.             
+  
+  Ltac estep_or_sstep :=
+    match goal with
+    | [ |- Csem2.step _ _ (Csem2.ExprState _ _ _ _ _ _ _ _) _ 
+                      (Csem2.ExprState _ _ _ _ _ _ _ _) ]=>
+        left
+    | [ |- Csem2.step _ _ _ _ _ ] =>
+        right
+    end.
+
+  Ltac doinv :=
+    match goal with
+    | [ H: match_cont (_ _) _ |- _ ] => inv H
+    | [ H: match_statement (_ _) _ |- _ ] => inv H
+    | [ H: match_statement CS1.Sskip _ |- _ ] => inv H
+    | [ H: match_expr (_ _) _ |- _ ] => inv H
+    | [ H: match_val _ _ |- _ ] => inv H
+    | [ H1: match_expr (?C1 ?expr1) ?expr2,
+          H2: match_ctx ?C1 ?C2 |- _ ] =>
+        apply (H2.(r C1 C2) expr1 expr2) in H1;
+        let a := fresh "a" in
+        let H3 := fresh "H" in
+        let H4 := fresh "H" in
+        destruct H1 as [a [H3 H4]]; subst expr2; inv H4; inv H1
+    | [ H1: match_env ?e1 ?e2,
+          H2: ?e1 ! ?x = _ |- _ ] =>
+        let H3 := fresh "H" in
+        pose proof (H1 x) as H3;
+        rewrite H2 in H3;
+        destruct (e2!x) eqn:?; inv H3; clear H2
+    | [ H1: match_tenv ?te1 ?te2,
+          H2: ?te1 ! ?b = ?a |- _ ] =>
+        let H3 := fresh "H" in
+        let v := fresh "v" in
+        let vt := fresh "vt" in
+        pose proof (H1 b) as H3; unfold M1.MD.TLib.atom in *;
+        rewrite H2 in H3; destruct te2!b as [[v vt]|] eqn:?; inv H3;
+        simpl in *; subst; clear H2
+    | [ H1: match_ctx ?C1 ?C2,
+          H2: Csem1.context ?k1 ?k2 ?C1 |- _ ] =>
+        assert (Csem2.context k1 k2 C2) by
+        (rewrite <- (H1.(closed_context C1 C2)); eauto);
+        clear H2
+    | [ H1: _ = ?C1 ?expr1,
+          H2: _ = ?C1 ?expr1 |- _ ] =>
+        rewrite <- H1 in H2; inv H2
+    end.
+  
+  Ltac use_ctx :=
+    match goal with
+    | [ H: match_ctx ?C1 ?C2 |- match_expr (?C1 _) (?C2 _) ] =>
+        apply (H.(closed_expr C1 C2))
+    end.
+
+  Lemma lred_transl :
+    forall e1 e2 lc C1 C2 expr1 expr2 pct1 pct2 te1 te2 m1 m2 expr1' te1' m1',
+      match_env e1 e2 ->
+      match_expr expr1 expr2 ->
+      match_tenv te1 te2 ->
+      match_ctx C1 C2 ->
+      (*match_mem m1 m2 ->*)
+      Csem1.lred ge1 ce e1 lc (C1 expr1) pct1 te1 m1 expr1' te1' m1' ->
+      exists expr2' te2' m2',
+        Csem2.lred ge2 ce e2 lc (C2 expr2) pct2 te2 m2 expr2' te2' m2' /\
+          match_expr expr1' expr2'. (* /\
+          match_tenv te1' te2'. /\
+                                 match_mem m1' m2'.*)
+  Proof.
+    intros. apply (H2.(closed_expr C1 C2)) in H0.
+    inv H3; inv H0; try congruence; repeat doinv;
+      repeat eexist'; deduce_match.
+    - eapply Csem2.red_var_tmp; eauto.
+    - eapply Csem2.red_var_local; eauto.
+    - eapply Csem2.red_var_global; eauto. admit.
+    - eapply Csem2.red_func; eauto. admit.
+    - eapply Csem2.red_ext_func; eauto. admit.
+    - eapply Csem2.red_builtin; eauto.
+    - eapply Csem2.red_deref.
+    - eapply Csem2.red_field_struct; eauto. reflexivity.
+    - eapply Csem2.red_field_union; eauto. reflexivity.
+  Admitted.
+
+  Lemma rred_transl :
+    forall e1 e2 lc C1 C2 expr1 expr2 pct1 pct2 te1 te2 m1 m2 pct1' expr1' te1' m1' tr1,
+      match_env e1 e2 ->
+      match_expr expr1 expr2 ->
+      match_tenv te1 te2 ->
+      match_ctx C1 C2 ->
+      (*match_mem m1 m2 ->*)
+      Csem1.rred ge1 ce lc pct1 (C1 expr1) te1 m1 tr1 pct1' expr1' te1' m1' ->
+      exists pct2' expr2' te2' m2' tr2,
+        Csem2.rred ge2 ce lc pct2 (C2 expr2) te2 m2 tr2 pct2' expr2' te2' m2' /\
+          match_expr expr1' expr2'. (* /\
+          match_tenv te1' te2'. /\
+                                 match_mem m1' m2'.*)
+  Proof.
+    intros. apply (H2.(closed_expr C1 C2)) in H0.
+    inv H3; inv H0; try congruence; repeat doinv; repeat eexist';
+      try (deduce_match; [| econstructor]);
+      try (econstructor; eauto; reflexivity; fail).
+    - econstructor. pose proof deref_loc_match. reflexivity. reflexivity.
+    - econstructor. admit. reflexivity.
+    - econstructor. admit. reflexivity.
+    - admit.
+    - admit.
+    - admit.
+    - admit.
+    - repeat econstructor; eauto. erewrite bool_val_eq in H5; eauto. constructor.
+    - repeat econstructor; eauto. erewrite bool_val_eq in H5; eauto. constructor.
+    - repeat econstructor. erewrite bool_val_eq in H5; eauto. constructor.
+    - erewrite bool_val_eq in H5; eauto. split. eapply Csem2.red_seqor_false; eauto.
+      reflexivity. constructor. auto. constructor.
+    - repeat econstructor. erewrite bool_val_eq in H5; eauto. constructor.
+      destruct b; auto.
+    - pose proof (sem_cast_match v2 v2 ty2 ty1 m3 m4).
+      rewrite H5 in H0.
+      destruct (CS2.Cop.sem_cast v2 ty2 ty1 m4) eqn:?;
+               unfold match_option_map in H0; unfold match_val in H0; try congruence.
+      econstructor; eauto. admit. reflexivity. reflexivity. admit.
+    - pose proof (sem_cast_match v2 v2 ty2 ty1 m1' m4).
+      rewrite H6 in H0.
+      destruct (CS2.Cop.sem_cast v2 ty2 ty1 m4) eqn:?;
+               unfold match_option_map in H0; unfold match_val in H0; try congruence.
+      econstructor; eauto. rewrite <- H0; eauto. reflexivity.
+    - deduce_match. econstructor. admit. reflexivity. reflexivity.
+      repeat econstructor. repeat econstructor.
+    - repeat econstructor; eauto.
+    - repeat econstructor.
+    - repeat econstructor.
+    - repeat econstructor. admit.
+    - repeat econstructor. admit.
+    - repeat econstructor; eauto.
+    - repeat econstructor; eauto.
+    - repeat econstructor.
+    - repeat econstructor.
+    - repeat econstructor.
+    - repeat econstructor.
+    - repeat econstructor. inv H7; eauto. eauto.
+    - pose proof (sem_cast_match v1 v1 ty1 ty2 m1' m4).
+      rewrite H5 in H0.
+      destruct (CS2.Cop.sem_cast v1 ty1 ty2 m4) eqn:?;
+               unfold match_option_map in H0; unfold match_val in H0; try congruence.
+      econstructor. rewrite <- H0; eauto. reflexivity.
+  Admitted.
   
   Theorem PolicyInsensitiveForward : forward_simulation sem1 sem2.
   Proof.
@@ -85,10 +719,58 @@ Module PolicyInsensitivity (Ptr: Pointer) (Pol: Policy)
                 is Csem2.state. Destruct on (initial_state s1) and construct an
                 s2 such that (final_state s2) but with other tags, so matching.*)
     - instantiate (1 := match_states). intros. inv H0.
-      inv H. inv H0. inv H0. eexists. eexists. intuition.
-      econstructor.
-      admit. (* Need to show that state is equivalent to Csem1.state and state0
-                is Csem2.state. Destruct and apply rules. *)
+      + inv H. inv H0.
+        inv H0; try (repeat doinv; eexists; eexists; intuition;
+                     [estep_or_sstep| |];
+                     repeat (econstructor; eauto); fail).
+        * repeat doinv. eexists. eexists.
+          intuition. estep_or_sstep. 2:econstructor; eauto.
+          -- econstructor. inv H11; try congruence.
+          -- repeat (econstructor; eauto).
+          -- econstructor.
+        * admit. (* do_free_variables match *)
+        * admit. (* do_free_variables match *)
+        * admit. (* do_free_variables match *)
+        * admit. (* do_free_variables match *)
+        * admit. (* find_label match *)
+      + inv H; inv H0.
+        * inv H15; pose proof (matching_ctx_matches C); repeat doinv;
+            try (deduce_match;
+                 [estep_or_sstep; repeat (econstructor; eauto)
+                 | use_ctx; econstructor ]; fail).
+          -- deduce_match. estep_or_sstep.
+             econstructor; eauto.
+             eapply Csem2.red_var_global. admit. admit. admit.
+          -- deduce_match.
+             estep_or_sstep.
+             econstructor; eauto.
+             eapply Csem2.red_func. admit. admit. admit.
+          -- deduce_match.
+             estep_or_sstep.
+             econstructor; eauto.
+             eapply Csem2.red_ext_func. admit. admit. admit.
+            admit.
+          -- admit.
+          -- admit.
+        * inv H15; pose proof (matching_ctx_matches C); repeat doinv.
+          -- deduce_match. estep_or_sstep. 
+            try (deduce_match;
+                 [estep_or_sstep; repeat (econstructor; eauto)
+                 | use_ctx; econstructor ]; fail).
+        replace (matching_ctx C) with C2 in H by auto.
+        match goal with
+        | [ H: Csem1.lred _ _ _ _ _ _ _ _ _ _ _ |- Csem2.estep _ _ _ _ _ ] =>
+            eapply Csem2.step_lred
+        end.
+        * inv H15.
+          -- econstructor.
+          deduce_state.
+              estep_or_sstep; repeat (econstructor; eauto)).
+        deduce_state. estep_or_sstep.
+      + admit.
+      + admit.
+      + admit.
+      + admit.
     Admitted.
   
 End PolicyInsensitivity.
